theories/Iris/Instance.v
@@ -46,7 +46,7 @@ From iris Require Import
      proofmode.tactics.
 
 From Katamaran Require Import
-     Iris.Model
+     Iris.Base
      Prelude
      Semantics
      Sep.Hoare
